wip

examples/low-level/crypto/Crypto.Symmetric.PRF.fst
@@ -240,54 +240,53 @@ private let lemma_modifies_ref (#t:Type) (r:HS.ref t) (rgn:HH.rid{rgn <> HS (r.i
 
 private let lemma_modifies_prf_raw (#a:Type) (#t:Type) (r:HS.ref a) (b:Buffer.buffer t)
   h0 h1 h2 : Lemma
-  (requires (HS.MkRef.id r <> Buffer.frameOf b /\ HS.modifies (Set.singleton (HS.MkRef.id r)) h0 h1
-    /\ HS (r.id `is_in` h0.h)
-    /\ HS.modifies_ref (HS.MkRef.id r) !{HS.as_ref r} h0 h1
+  (requires (
+    let rr = HS.MkRef.id r in
+    let rb = Buffer.frameOf b in 
+      rr <> rb 
+    /\ HS.modifies (Set.singleton rr) h0 h1
+    /\ HS (rr `is_in` h0.h)
+    /\ HS.modifies_ref rr !{HS.as_ref r} h0 h1
     /\ Buffer.live h0 b
     /\ HS (h1.tip == h0.tip)
     /\ Buffer.modifies_1 b h1 h2))
-  (ensures  (HS.modifies (Set.union (Set.singleton (HS.MkRef.id r)) (Set.singleton (Buffer.frameOf b))) h0 h2
-    /\ Buffer.modifies_buf_1 (Buffer.frameOf b) b h0 h2
-    /\ HS.modifies_ref (HS (r.id)) (TSet.singleton (FStar.Heap.Ref (HS.as_ref r))) h0 h2))
-    = Buffer.lemma_reveal_modifies_1 b h1 h2;
-      let rr = HS.MkRef.id r in
-      let rb = Buffer.frameOf b in 
-      let rgns = Set.union (Set.singleton rr) (Set.singleton #HH.rid rb) in 
-      (* cut (HS.modifies rgns h0 h2); *)
-      cut (HS.modifies_ref rr (TSet.singleton (FStar.Heap.Ref (HS.as_ref r))) h0 h1);
-      cut (HS.modifies_ref rr (TSet.singleton (FStar.Heap.Ref (HS.as_ref r))) h1 h2);
-      lemma_modifies_buf_1 b rr h0 h1;
-      lemma_modifies_ref r rb h1 h2
+  (ensures  (
+    let rr = HS.MkRef.id r in
+    let rb = Buffer.frameOf b in 
+      HS.modifies (Set.union (Set.singleton rr) (Set.singleton rb)) h0 h2
+    /\ Buffer.modifies_buf_1 rb b h0 h2
+    /\ HS.modifies_ref rr (TSet.singleton (FStar.Heap.Ref (HS.as_ref r))) h0 h2)) = 
+    
+    Buffer.lemma_reveal_modifies_1 b h1 h2;
+    let rr = HS.MkRef.id r in
+    let rb = Buffer.frameOf b in 
+    //let rgns = Set.union (Set.singleton rr) (Set.singleton #HH.rid rb) in 
+    //cut (HS.modifies rgns h0 h2);
+    //cut (HS.modifies_ref rr (TSet.singleton (FStar.Heap.Ref (HS.as_ref r))) h0 h1);
+    //cut (HS.modifies_ref rr (TSet.singleton (FStar.Heap.Ref (HS.as_ref r))) h1 h2);
+    lemma_modifies_buf_1 b rr h0 h1;
+    lemma_modifies_ref r rb h1 h2
 
+let modifies_table_buffer_1 #i (t:state i) b h0 h1 = 
+  Buffer.live h1 b /\ 
+  (if prf i then ( 
+    let r = itable i t in 
+    let rb = Buffer.frameOf b in 
+    // can't use !{ t.rgn, rb}, why?
+    let rgns = Set.union (Set.singleton #HH.rid t.rgn) (Set.singleton #HH.rid rb) in 
+    HS.modifies rgns h0 h1 /\ 
+    HS.modifies_ref t.rgn (TSet.singleton (FStar.Heap.Ref (HS.as_ref r))) h0 h1 /\
+    Buffer.modifies_buf_1 rb b h0 h1 )
+  else
+    Buffer.modifies_1 b h0 h1)
 
 // real case + real use of memoized PRF output.
 private val prf_raw: 
   i:id -> t:state i -> x:domain{x.ctr <> 0ul /\ ~(safeId i)} -> l:u32 {l <=^ blocklen} -> 
   output:lbuffer (v l) {Buffer.frameOf output <> t.rgn} -> ST unit
   (requires (fun h0 -> Buffer.live h0 output))
-  (ensures (fun h0 _ h1 -> 
-    Buffer.live h1 output /\ 
-    (if prf i then ( (*True
-      (
-      // 16-10-08 this is gross; we need nicer libraries!
-      // I just want to write modifies !{ itable i t, output } h0 h1
-      // we should never have to refer to several of H, HH, HS, HST (and maybe Buffer) at the same time!
-      // can't get any concrete syntax for sets to work below.
-      //
-      // Temporarily giving up on hybrid modifies posts in the rest of the file.
-      // *)
-      let r = itable i t in 
-      let rb = Buffer.frameOf output in 
-      // can't use !{ t.rgn, rb}, why?
-      let rgns = Set.union (Set.singleton #HH.rid t.rgn) (Set.singleton #HH.rid rb) in 
-      Buffer.live h1 output /\ 
-      HS.modifies rgns h0 h1 /\ 
-      HS.modifies_ref t.rgn (TSet.singleton (FStar.Heap.Ref (HS.as_ref r))) h0 h1 /\
-      Buffer.modifies_buf_1 rb output h0 h1 )
-      (* *) 
-    else
-      Buffer.modifies_1 output h0 h1
-    )))
+  (ensures (fun h0 _ h1 -> modifies_table_buffer_1 t output h0 h1)) 
+
 let prf_raw i t x l output = 
   if prf i then (
     let r = itable i t in 
@@ -296,22 +295,21 @@ let prf_raw i t x l output =
     let block = 
       match find_blk contents x with 
       | Some block -> (
-          cut (HS.modifies (Set.singleton (HS.MkRef.id r)) h0 h0);
+          //cut (HS.modifies (Set.singleton (HS.MkRef.id r)) h0 h0);
           block)
       | None ->
           let block = random blocklen in 
-          let h = HST.get() in
+          // let h = HST.get() in
           r := SeqProperties.snoc contents (Entry x block);
-          let h' = HST.get() in
-          assert(h' == HS.upd h r (SeqProperties.snoc contents (Entry x block)));
-          cut (HS.modifies (Set.singleton (HS.MkRef.id r)) h h');
+          // let h' = HST.get() in
+          // assert(h' == HS.upd h r (SeqProperties.snoc contents (Entry x block)));
+          // cut (HS.modifies (Set.singleton (HS.MkRef.id r)) h h');
           block in
     let h1 = HST.get() in
-    cut (HS.modifies (Set.singleton (HS.MkRef.id r)) h0 h1);
+    // cut (HS.modifies (Set.singleton (HS.MkRef.id r)) h0 h1);
     store_bytes l output (Seq.slice block 0 (v l));
     let h2 = HST.get() in
-    lemma_modifies_prf_raw r output h0 h1 h2
-    )
+    lemma_modifies_prf_raw r output h0 h1 h2)
   else
     getBlock t x l output
  
